\formtitle{Méthodes itératives}

Principe commun : 

\begin{enumerate}
    \item Init : $x^{(0)}$ à 0 
    \item Itération : $x^{(k)} \leftarrow x^{(k-1)}$
    \item Jusqu'à condition d'arrêt
\end{enumerate}

\formtitle{Méthodes de Jacobi}

$$x_i^{(k+1)} = \frac{1}{a_{ii}} \left( b_i - \sum_{j=1, j\neq i}^n a_{ij} x_j^{(k)} \right) \quad i=1,\dots,n$$


\formtitle{Méthodes de Gauss-Seidel}

$$x_i^{(k+1)} = \frac{1}{a_{ii}} \left( b_i - \sum_{j=1}^{i-1} a_{ij} x_j^{(k+1)} - \sum_{j=i+1}^n a_{ij} x_j^{(k)} \right) \quad i=1,\dots,n$$

Exemple :
\[
\begin{bmatrix}
    4&-1&1 \\
    -1&4&-2 \\
    1&-2&4\\ 
\end{bmatrix}
\begin{bmatrix}
    x_1 \\
    x_2 \\
    x_3 \\
\end{bmatrix}
=
\begin{bmatrix}
    12 \\
    -1 \\
    5 \\
\end{bmatrix}
\]

Jacobi :

\[
\vec{x}^{(1)} = \begin{bmatrix}
    3 \\
    -0.25 \\
    1.25 \\
\end{bmatrix}
\Rightarrow
\vec{x}^{(2)} = \begin{bmatrix}
    2.625 \\
    1.125 \\
    0.375 \\
\end{bmatrix}
\Rightarrow
\vec{x}^{(3)} = \begin{bmatrix}
    3.187 \\
    0.593 \\
    1.156 \\
\end{bmatrix}
\]

Gauss-Seidel :

\[
\vec{x}^{(1)} = \begin{bmatrix}
    3 \\
    0.50 \\
    0.75 \\
\end{bmatrix}
\Rightarrow
\vec{x}^{(2)} = \begin{bmatrix}
    2.9375 \\
    0.8594 \\
    0.9453 \\
\end{bmatrix}
\Rightarrow
\vec{x}^{(3)} = \begin{bmatrix}
    2.9785 \\
    0.9678 \\
    0.9890 \\
\end{bmatrix}
\]

\formtitle{Méthodes de gradient}

Algorithme de la plus grande pente :

\begin{enumerate}
    \item Init : $x^{(0)}$ dans $\mathbb{R}^n$
    \item Itération : 
        \begin{enumerate}
            \item $\vec{d}_k = - \nabla G(x^{(k)}) = \vec{b} -A\vec{x}_{k} = \vec{r}_k$
            \item $a_k = \cfrac{\vec{d}_k^T \vec{r}_k}{\vec{d}_k^T A \vec{d}_k} = \cfrac{\vec{r}_k^T \vec{r}_k}{\vec{r}_k^T A \vec{r}_k}$
            \item $x^{(k+1)} = x^{(k)} + a_k \vec{d}_k$
        \end{enumerate}
\end{enumerate}

\formtitle{Méthodes de gradient conjugué}

\begin{enumerate}
    \item Init : $x^{(0)}$ dans $\mathbb{R}^n$
    \item initialiser $\vec{r}_0 = b - Ax^{(0)}$ et $\vec{d}_0 = \vec{r}_0$
    \item Itération : 
        \begin{enumerate}
            \item $\vec{d}_k = - \nabla G(x^{(k)}) = \vec{b} -A\vec{x}_{k} = \vec{r}_k$
            \item $a_k = \cfrac{\vec{d}_k^T \vec{r}_k}{\vec{d}_k^T A \vec{d}_k}$
            \item $x^{(k+1)} = x^{(k)} + a_k \vec{d}_k$
            \item $\vec{r}_{k+1} = \vec{r}_k + a_k A \vec{d}_k$
            \item $\beta_{k+1} = \cfrac{\vec{r}_{k+1}^T \vec{r}_{k+1}}{\vec{r}_k^T \vec{r}_k}$
            \item $\vec{d}_{k+1} = - \vec{r}_{k+1} + \beta_{k+1} \vec{d}_k$
        \end{enumerate}
\end{enumerate}